src/common/Nemonuri.Unique.IntegerIntervals.fst
@@ -1,0 +1,59 @@
+module Nemonuri.Unique.IntegerIntervals
+
+module U = Nemonuri.Unique
+module I = FStar.IntegerIntervals
+
+let is_restricted
+  (imin: int) (emax: int) 
+  (refiner: (I.interval imin emax) -> Tot bool)
+  =
+  forall (x:int). 
+    {:pattern (I.interval_condition imin emax x) \/ (refiner x)}
+    (I.interval_condition imin emax x) ==> ~(refiner x)
+
+let is_exist
+  (imin: int) (emax: int) 
+  (refiner: (I.interval imin emax) -> Tot bool)
+  =
+  exists (x:int). 
+    {:pattern (I.interval_condition imin emax x) \/ (refiner x)}
+    (I.interval_condition imin emax x) /\ (refiner x)
+
+noeq
+type t = {
+  imin: int;
+  emax: int;
+  refiner: (I.interval imin emax) -> Tot bool;
+  witness: I.interval imin emax;
+  lemma_min_restricted: squash (is_restricted imin witness refiner);
+  lemma_max_restricted: squash (is_restricted (witness+1) emax refiner);
+  lemma_exists: squash (is_exist imin emax refiner);
+}
+
+let lemma_unique (u:t)
+  : Lemma ((U.singleton_predicate u.refiner) /\ (u.refiner u.witness)) =
+  ()
+
+let to_unique (u:t) = U.intro_unique u.refiner u.witness
+
+let to_prop (u:t) : Tot Type0 =
+  (is_restricted u.imin u.witness u.refiner) /\
+  (is_restricted (u.witness+1) u.emax u.refiner) /\
+  (is_exist u.imin u.emax u.refiner) /\
+  (U.singleton_predicate u.refiner) /\ (u.refiner u.witness)
+
+let create_prop
+  (imin: int)
+  (emax: int)
+  (refiner: (I.interval imin emax) -> Tot bool)
+  (witness: I.interval imin emax)
+  (lemma_min_restricted: squash (is_restricted imin witness refiner))
+  (lemma_max_restricted: squash (is_restricted (witness+1) emax refiner))
+  (lemma_exists: squash (is_exist imin emax refiner))
+  : Tot Type0 =
+  to_prop {
+    imin=imin; emax=emax; refiner=refiner; witness=witness;
+    lemma_min_restricted=lemma_min_restricted;
+    lemma_max_restricted=lemma_max_restricted;
+    lemma_exists=lemma_exists;
+  }
