src/common/Nemonuri.Unique.fst
@@ -1,0 +1,60 @@
+module Nemonuri.Unique
+
+(*
+   Uniqueness quantification
+   - https://en.wikipedia.org/wiki/Uniqueness_quantification
+*)
+
+let singleton_predicate (#dom_t:eqtype) (refiner:dom_t -> Tot bool) =
+  exists (x:dom_t). (forall (y:dom_t). (refiner y) <==> (y = x))
+
+type singleton_t (dom_t:eqtype) = p:(dom_t -> Tot bool){singleton_predicate p}
+
+
+let intro_singleton 
+  (#dom_t:eqtype) (refiner:dom_t -> Tot bool) (w:dom_t)
+  : Pure (singleton_t dom_t)
+    (requires (forall (w1:dom_t). (refiner w1) <==> (w1 = w)))
+    (ensures fun _ -> true)
+  =
+  refiner
+
+let intro_singleton2
+  (#dom_t:eqtype) (refiner:dom_t -> Tot bool) (w:dom_t)
+  : Pure (singleton_t dom_t)
+    (requires (forall (w1 w2:dom_t). ((refiner w1) /\ (refiner w2)) ==> (w1 = w2)) /\ (refiner w))
+    (ensures fun _ -> true)
+  =
+  refiner
+
+//let unique_predicate (#dom_t:eqtype) (singleton:singleton_t dom_t) (witness:dom_t) : Tot bool = singleton witness
+
+type witness_t (#dom_t:eqtype) (singleton:singleton_t dom_t) = x:dom_t{singleton x}
+
+noeq
+type t (dom_t:eqtype) = {
+  singleton: singleton_t dom_t;
+  witness: witness_t singleton
+}
+
+let intro_unique
+  (#dom_t:eqtype) (refiner:dom_t -> Tot bool) (w:dom_t)
+  : Pure (t dom_t)
+    (requires (forall (w1:dom_t). (refiner w1) <==> (w1 = w)))
+    (ensures fun _ -> true)
+  =
+  {
+    singleton = intro_singleton refiner w;
+    witness = w
+  }
+
+let intro_unique2
+  (#dom_t:eqtype) (refiner:dom_t -> Tot bool) (w:dom_t)
+  : Pure (t dom_t)
+    (requires (forall (w1 w2:dom_t). ((refiner w1) /\ (refiner w2)) ==> (w1 = w2)) /\ (refiner w))
+    (ensures fun _ -> true)
+  =
+  {
+    singleton = intro_singleton2 refiner w;
+    witness = w
+  }
